CleanQ/CleanQ_RBModel.thy
@@ -25,7 +25,7 @@ theory CleanQ_RBModel
   imports Main "../Simpl/Vcg"  "../Complx/OG_Hoare" CleanQ_ListModel CleanQ_RB
 (*>*)  
 begin
-
+declare[[show_types]]
 
 (* ==================================================================================== *)
 subsection \<open>CleanQ Abstract Ring Buffer Model State\<close>
@@ -219,28 +219,36 @@ text \<open>
   we up to now implicitly used. \<close>
 definition frame_rb_weak_x :: "'a CleanQ_RB_State \<Rightarrow> 'a CleanQ_RB_State \<Rightarrow> bool"
   where "frame_rb_weak_x st' st \<longleftrightarrow> rSX st = rSX st' \<and> frame_rb_weak_left (rTXY st') (rTXY st) 
-                                    \<and> frame_rb_weak_right (rTYX st') (rTYX st) \<and>
-                                    (\<exists>\<delta>txy \<delta>tyx. rSY st' = set (\<delta>txy) \<union> rSY st - (set \<delta>tyx))" 
+                                    \<and> frame_rb_weak_right (rTYX st') (rTYX st) \<and> 
+                                    (rSY st' = set (rb_delta_tail_st (rTXY st') (rTXY st)) \<union> 
+                                     rSY st - set (rb_delta_head_st (rTYX st') (rTYX st)))" 
 
 definition frame_rb_weak_y :: "'a CleanQ_RB_State \<Rightarrow> 'a CleanQ_RB_State \<Rightarrow> bool"
   where "frame_rb_weak_y st' st \<longleftrightarrow> rSY st = rSY st' \<and> frame_rb_weak_left (rTYX st') (rTYX st) \<and>
                                     frame_rb_weak_right (rTXY st') (rTXY st) \<and>
-                                    (\<exists>\<delta>txy \<delta>tyx. rSX st' = set (\<delta>tyx) \<union> rSX st - (set \<delta>txy))"
+                                    (rSX st' = set (rb_delta_tail_st (rTYX st') (rTYX st)) \<union> 
+                                     rSX st - set (rb_delta_head_st (rTXY st') (rTXY st)))"
 
 lemma frame_rb_s_w_x:
  "frame_rb_strong st' st \<Longrightarrow> frame_rb_weak_x st' st"
   unfolding frame_rb_weak_x_def frame_rb_strong_def frame_rb_weak_left_def
-  frame_rb_weak_right_def
-  by (metis Diff_empty I4_rb_valid.elims(2) add.right_neutral list.set(1) rb_valid_def 
-      rb_valid_ptr_def sup_bot.left_neutral zero_le)
+  frame_rb_weak_right_def rb_delta_tail_st_def rb_delta_head_st_def
+  by (metis Diff_empty I4_rb_valid.elims(2) Nat.add_0_right Un_empty_left diff_self_eq_0 le0 
+      le_refl list.map(1) list.set(1) rb_delta_head_def rb_delta_tail_def rb_incr_head_n_delta_def 
+      rb_incr_head_n_delta_map_def rb_incr_tail_n_delta_def rb_incr_tail_n_delta_map_def rb_valid_def 
+      rb_valid_ptr_def take0) 
+
 
 
 lemma frame_rb_s_w_y:
   "frame_rb_strong dev' dev \<Longrightarrow> frame_rb_weak_y dev' dev"
   unfolding frame_rb_weak_y_def frame_rb_strong_def frame_rb_weak_left_def
-  frame_rb_weak_right_def
-  by (metis Diff_empty I4_rb_valid.elims(2) add.right_neutral list.set(1) 
-      rb_valid_def rb_valid_ptr_def sup_bot.left_neutral zero_le)
+  frame_rb_weak_right_def rb_delta_tail_st_def rb_delta_head_st_def
+  by (metis Diff_empty I4_rb_valid.elims(2) add.commute add.left_neutral diff_self_eq_0 
+      le_refl list.map(1) list.set(1) rb_delta_head_def rb_delta_tail_def rb_incr_head_n_delta_def 
+      rb_incr_head_n_delta_map_def rb_incr_tail_n_delta_def rb_incr_tail_n_delta_map_def rb_valid_def 
+      rb_valid_ptr_def sup_bot.left_neutral take0 zero_le)
+
 
 (* ------------------------------------------------------------------------------------ *)
 subsubsection \<open>All CleanQ RB Invariants\<close>
@@ -267,162 +275,28 @@ lemma CleanQ_RB_Invariants_List_Invariants:
 text \<open>In order to show that the RB weak frame condition refines the List weak frame condition we need some
       helper lemmas.\<close>
 
-lemma frame_weak_x_exists_tl_delta: 
-  assumes Inv: "CleanQ_RB_Invariants K rb'" and
-          frame: "frame_rb_weak_x rb' rb"
-  shows"\<exists>\<delta>aB. map (the \<circ> ring (rTXY rb')) (rb_valid_entries (rTXY rb')) =
-          \<delta>aB @ map (the \<circ> ring (rTXY rb)) (rb_valid_entries (rTXY rb))"
-  using Inv frame rb_weak_delta_tail_n 
-proof -
-    from frame obtain \<delta>tl 
-      where tl: "\<delta>tl \<le> rb_can_incr_tail_n_max (rTXY rb') \<and> 
-           (if tail (rTXY rb') + \<delta>tl < size (rTXY rb') then tail (rTXY rb') + \<delta>tl
-           else (tail (rTXY rb') + \<delta>tl) mod size (rTXY rb')) = tail (rTXY rb)"
-    unfolding frame_rb_weak_x_def frame_rb_weak_left_def frame_rb_weak_right_def
-    by blast
-
-  from frame have incr: "rb_can_incr_tail_n \<delta>tl (rTXY rb')"
-    by (simp add: rb_can_incr_tail_max_implies_can_incr tl) 
-
-  from assms have delta: "rb_valid_entries (rTXY rb') = (rb_incr_tail_n_delta \<delta>tl (rTXY rb')) @ (rb_valid_entries (rTXY rb))"
-      using tl incr using rb_weak_delta_tail_n
-      using frame_rb_weak_x_def
-      by (metis (no_types, lifting) CleanQ_RB.ext_inject CleanQ_RB.surjective CleanQ_RB.update_convs(3) 
-          mod_less rb_incr_tail_n_def) 
-
-  show ?thesis using incr tl delta
-    by (metis (no_types, hide_lams) frame frame_rb_weak_left_def frame_rb_weak_x_def map_append) 
-qed
-
 lemma frame_weak_x_tl_delta: 
   assumes Inv: "CleanQ_RB_Invariants K rb'" and
-          frame: "frame_rb_weak_x rb' rb" and
-          incr: "rTXY rb = rb_incr_tail_n n (rTXY rb')" and
-          can_incr: "rb_can_incr_tail_n n (rTXY rb')" 
-  shows"map (the \<circ> ring (rTXY rb')) (rb_valid_entries (rTXY rb')) =
-        map (the \<circ> ring (rTXY rb')) (rb_incr_tail_n_delta n (rTXY rb')) @ map (the \<circ> ring (rTXY rb)) (rb_valid_entries (rTXY rb))"
-  using Inv frame rb_weak_delta_tail_n 
-proof -
-  from frame have st: "rTXY rb = rb_incr_tail_n n (rTXY rb')" 
-    unfolding frame_rb_weak_x_def frame_rb_weak_left_def
-    using incr by blast 
-
-  from assms have delta: "rb_valid_entries (rTXY rb') = (rb_incr_tail_n_delta n (rTXY rb')) @ (rb_valid_entries (rTXY rb))"
-      using can_incr st using rb_weak_delta_tail_n
-      using frame_rb_weak_x_def
-      by (simp add: frame_rb_weak_x_def rb_weak_delta_tail_n)
-      
-  from assms delta have drop:"rb_valid_entries (rTXY rb) = drop n (rb_valid_entries (rTXY rb'))"
-    by (metis append_take_drop_id rb_incr_tail_n_delta_def same_append_eq) 
-     
-  from frame have valid: "rb_valid (rTXY rb) \<and> rb_valid (rTXY rb')"
-     by (simp add: frame_rb_weak_left_def frame_rb_weak_x_def)
-
-  from drop valid can_incr st rb_ring_map_drop_eq
-  have core: "map (the \<circ> ring (rTXY rb)) (rb_valid_entries (rTXY rb)) = (map (the \<circ> ring (rTXY rb')) (drop n (rb_valid_entries (rTXY rb'))))"
-    by (simp add: rb_ring_map_drop_eq valid) 
-
-  from assms have eq: "map (the \<circ> ring (rTXY rb')) (drop n (rb_valid_entries (rTXY rb'))) = map (the \<circ> ring (rTXY rb)) (rb_valid_entries (rTXY rb))"
-    using core by auto
-
-  from assms have eq2: "map (the \<circ> ring (rTXY rb')) (rb_valid_entries (rTXY rb')) =
-                       map (the \<circ> ring (rTXY rb')) (take n (rb_valid_entries (rTXY rb'))) @ map (the \<circ> ring (rTXY rb')) (drop n (rb_valid_entries (rTXY rb')))"
-    using drop rb_valid_tl_delta_take_drop by blast
-
-  from assms have eq3: "map (the \<circ> ring (rTXY rb')) (rb_valid_entries (rTXY rb)) = map (the \<circ> ring (rTXY rb)) (rb_valid_entries (rTXY rb))"
-    using drop eq by auto
-   
-  show ?thesis
-    by (simp add: delta eq3) 
-qed
-
-
-lemma frame_weak_x_exists_hd_delta:
-  assumes Inv: "CleanQ_RB_Invariants K rb'" and
           frame: "frame_rb_weak_x rb' rb"
-  shows"\<exists>\<delta>Bc. map (the \<circ> ring (rTYX rb')) (rb_valid_entries (rTYX rb')) @ \<delta>Bc =
-                 map (the \<circ> ring (rTYX rb)) (rb_valid_entries (rTYX rb))"
-  using Inv frame rb_weak_delta_head_n
-proof -
-    from frame obtain \<delta>hd
-    where hd: "\<delta>hd \<le> rb_can_incr_head_n_max (rTYX rb') \<and>
-           (if head (rTYX rb') + \<delta>hd < size (rTYX rb') then head (rTYX rb') + \<delta>hd
-           else (head (rTYX rb') + \<delta>hd) mod size (rTYX rb')) = head (rTYX rb)"
-    unfolding frame_rb_weak_x_def frame_rb_weak_left_def frame_rb_weak_right_def
-    by blast
-
-  from frame have valid: "rb_valid_ptr (rTYX rb')"
-    unfolding frame_rb_weak_x_def frame_rb_weak_right_def rb_valid_def
-    by blast
-
-  from hd have incr: "rb_can_incr_head_n \<delta>hd (rTYX rb')"
-    using valid rb_can_incr_head_max_implies_can_incr
-    by blast
-
-  from frame hd incr have hd2: "head (rTYX rb) = head (rb_incr_head_n \<delta>hd (rTYX rb'))"
-    unfolding frame_rb_weak_x_def 
-    by (metis CleanQ_RB.cases_scheme CleanQ_RB.select_convs(2) CleanQ_RB.update_convs(2) 
-        mod_less rb_incr_head_n_def)
-
-  from frame have delta: "rb_valid_entries (rTYX rb') @ (rb_incr_head_n_delta \<delta>hd (rTYX rb')) = rb_valid_entries (rTYX rb)"
-    using hd incr rb_weak_delta_head_n unfolding frame_rb_weak_x_def
-    using \<open>head (rTYX rb) = head (rb_incr_head_n \<delta>hd (rTYX rb'))\<close> by fastforce
-
-  show ?thesis using delta
-    by (metis (no_types, hide_lams) frame frame_rb_weak_right_def frame_rb_weak_x_def map_append) 
-   
-qed
-
+  shows"map (the \<circ> ring (rTXY rb')) (rb_valid_entries (rTXY rb')) =
+        rb_delta_tail_st (rTXY rb') (rTXY rb) @ map (the \<circ> ring (rTXY rb)) (rb_valid_entries (rTXY rb))"
+  unfolding rb_delta_tail_st_def rb_incr_tail_n_delta_map_def rb_incr_tail_n_delta_def
+  by (metis (no_types, hide_lams) frame frame_rb_weak_x_def rb_delta_tail_incr rb_delta_tail_st_def 
+      rb_incr_tail_n_delta_def rb_incr_tail_n_delta_map_def) 
 
 lemma frame_weak_x_hd_delta:
   assumes Inv: "CleanQ_RB_Invariants K rb'" and
-          frame: "frame_rb_weak_x rb' rb" and
-          incr: "rTYX rb = rb_incr_head_n n (rTYX rb')" and
-          can_incr: "rb_can_incr_head_n n (rTYX rb')" 
-  shows"map (the \<circ> ring (rTYX rb')) (rb_valid_entries (rTYX rb')) @ map (the \<circ> ring (rTYX rb)) (rb_incr_head_n_delta n (rTYX rb')) =
-        map (the \<circ> ring (rTYX rb)) (rb_valid_entries (rTYX rb))"
-  using assms rb_weak_delta_head_n 
-  unfolding frame_rb_weak_x_def
-proof -
-  assume a1: "rSX rb = rSX rb' \<and> frame_rb_weak_left (rTXY rb') (rTXY rb) \<and> frame_rb_weak_right (rTYX rb') (rTYX rb) \<and> (\<exists>\<delta>txy \<delta>tyx. rSY rb' = set \<delta>txy \<union> rSY rb - set \<delta>tyx)"
-  have "ring (rTYX rb) = ring (rTYX rb')"
-    by (simp add: incr rb_incr_head_n_ring)
-  then show ?thesis
-    using a1 can_incr incr rb_weak_delta_head_n by fastforce
-qed
-
-(*
-lemma frame_weak_x_exists_txy_delta:
-  assumes Inv: "CleanQ_RB_Invariants K rb'" and
           frame: "frame_rb_weak_x rb' rb"
-  shows "\<exists>\<delta>aB. (\<exists>\<delta>Bc. rSY rb' \<union> set \<delta>aB = set \<delta>Bc \<union> rSY rb \<and>
-                 rSY rb \<inter> set \<delta>Bc = {} \<and> distinct \<delta>Bc)"
-  using assms unfolding frame_rb_weak_x_def
-  by (metis Diff_disjoint Un_Diff_Int Un_Diff_cancel2 finite_Diff finite_Int 
-      finite_distinct_list finite_set)
-
-lemma frame_weak_x_txy_delta:
-  assumes Inv: "CleanQ_RB_Invariants K rb'" and
-          xy: "\<delta>xy = map (the \<circ> ring (rTYX rb')) (rb_incr_tail_n_delta \<delta>tl (rTXY rb'))" and
-          yx: "\<delta>yx = map (the \<circ> ring (rTYX rb)) (rb_incr_head_n_delta \<delta>hd (rTXY rb'))" and
-          frame: "frame_rb_weak_x rb' rb" 
-  shows "rSY rb' \<union> set \<delta>xy = set \<delta>yx \<union> rSY rb \<and> rSY rb \<inter> set \<delta>yx = {} \<and> distinct \<delta>xy"
-proof -
-  from Inv xy have "set \<delta>xy \<subseteq> rSX rb" 
-    apply simp unfolding CleanQ_RB_list_def 
-
-  from Inv xy have "distinct \<delta>xy"
-    apply simp 
-
-
-qed
-*)
-
-text \<open>Finally we show that the RB weak frame condition refines the List weak frame condition.\<close>
-
+  shows"map (the \<circ> ring (rTYX rb')) (rb_valid_entries (rTYX rb')) @ rb_delta_head_st (rTYX rb') (rTYX rb) =
+        map (the \<circ> ring (rTYX rb)) (rb_valid_entries (rTYX rb))"
+  unfolding rb_delta_head_st_def rb_incr_head_n_delta_map_def rb_incr_head_n_delta_def
+  using frame rb_delta_head_incr unfolding frame_rb_weak_x_def
+  by (metis rb_delta_head_st_def rb_incr_head_n_delta_def rb_incr_head_n_delta_map_def) 
+  
 (*
+text \<open>Finally we show that the RB weak frame condition refines the List weak frame condition.\<close>
 lemma frame_rb_weak_x_list_weak:
-  fixes rb rb' K \<delta>hd \<delta>tl
+  fixes rb rb' K
   assumes I1: "CleanQ_RB_Invariants K rb'"
       and frame: "frame_rb_weak_x rb' rb"
     shows "frame_list_weak (lTXY (CleanQ_RB2List rb'), lSY (CleanQ_RB2List rb'), lTYX (CleanQ_RB2List rb'), lSX (CleanQ_RB2List rb')) 
@@ -434,60 +308,25 @@ proof -
     by (metis frame frame_rb_weak_x_def) 
   show " \<And>x. x \<in> rSX rb \<Longrightarrow> x \<in> rSX rb'"
     by (metis frame frame_rb_weak_x_def)
+  show "\<exists>\<delta>aB::'a list.
+       map (the \<circ> ring (rTXY rb')) (rb_valid_entries (rTXY rb')) = \<delta>aB @ map (the \<circ> ring (rTXY rb)) (rb_valid_entries (rTXY rb)) \<and>
+       (\<exists>\<delta>Bc::'a list.
+           rSY rb' \<union> set \<delta>aB = set \<delta>Bc \<union> rSY rb \<and>
+           map (the \<circ> ring (rTYX rb')) (rb_valid_entries (rTYX rb')) @ \<delta>Bc = map (the \<circ> ring (rTYX rb)) (rb_valid_entries (rTYX rb)) \<and> rSY rb \<inter> set \<delta>Bc = {} \<and> distinct \<delta>Bc)"
+  using frame unfolding frame_rb_weak_x_def frame_rb_weak_left_def
+proof
 
-  from frame obtain \<delta>hd \<delta>tl
-    where hd: "\<delta>hd \<le> rb_can_incr_head_n_max (rTYX rb') \<and>
-           (if head (rTYX rb') + \<delta>hd < size (rTYX rb') then head (rTYX rb') + \<delta>hd
-           else (head (rTYX rb') + \<delta>hd) mod size (rTYX rb')) = head (rTYX rb)"
-      and tl: "\<delta>tl \<le> rb_can_incr_tail_n_max (rTXY rb') \<and> 
-           (if tail (rTXY rb') + \<delta>tl < size (rTXY rb') then tail (rTXY rb') + \<delta>tl
-           else (tail (rTXY rb') + \<delta>tl) mod size (rTXY rb')) = tail (rTXY rb)"
-    unfolding frame_rb_weak_x_def frame_rb_weak_left_def frame_rb_weak_right_def
-    by blast
+  define \<delta>xy where "\<delta>xy = rb_delta_tail_st (rTXY rb') (rTXY rb)"
+  define \<delta>yx where "\<delta>yx = rb_delta_head_st (rTYX rb') (rTYX rb)"
 
-  from assms have rb: "rTXY rb = rb_incr_tail_n \<delta>tl (rTXY rb')"
-    by (metis (no_types, lifting) CleanQ_RB.select_convs(3) CleanQ_RB.surjective CleanQ_RB.update_convs(3) 
-        frame_rb_weak_left_state frame_rb_weak_x_def mod_less rb_can_incr_tail_max_implies_can_incr rb_incr_tail_n_def tl)
+  have "map (the \<circ> ring (rTXY rb')) (rb_valid_entries (rTXY rb')) = \<delta>xy @ map (the \<circ> ring (rTXY rb)) (rb_valid_entries (rTXY rb))"
+    using I1 \<delta>xy_def frame frame_weak_x_tl_delta by blast
 
-  from rb have incr_tl: "rb_can_incr_tail_n \<delta>tl (rTXY rb')"
-    using rb_can_incr_tail_n_lt_max tl by blast
-
-  from assms incr_tl have rb_tl: "rTXY rb = rb_incr_tail_n \<delta>tl (rTXY rb')"
-    using rb by blast
-   
-  from rb have incr_hd: "rb_can_incr_head_n \<delta>hd (rTYX rb')"
-    by (meson CleanQ_RB_Invariants.elims(2) I1 I4_rb_valid.elims(2) hd rb_can_incr_head_max_implies_can_incr
-        rb_valid_def)
-
-  from assms incr_hd have rb_hd: "rTYX rb = rb_incr_head_n \<delta>hd (rTYX rb')"
-  proof -
-    have "(head (rTYX rb') + \<delta>hd) mod size (rTYX rb') = head (rTYX rb)"
-      by (metis (no_types) hd mod_less)
-    then show ?thesis
-      by (metis (no_types) CleanQ_RB.simps(2) CleanQ_RB.surjective CleanQ_RB.update_convs(2) frame frame_rb_weak_right_state frame_rb_weak_x_def incr_hd rb_incr_head_n_def)
-  qed
-
-  from assms incr_hd rb_hd incr_tl rb_tl frame_weak_x_hd_delta 
-  show "\<exists>\<delta>aB. map (the \<circ> ring (rTXY rb')) (rb_valid_entries (rTXY rb')) = \<delta>aB @ map (the \<circ> ring (rTXY rb)) (rb_valid_entries (rTXY rb)) \<and>
-          (\<exists>\<delta>Bc. rSY rb' \<union> set \<delta>aB = set \<delta>Bc \<union> rSY rb \<and>
-                 map (the \<circ> ring (rTYX rb')) (rb_valid_entries (rTYX rb')) @ \<delta>Bc = map (the \<circ> ring (rTYX rb)) (rb_valid_entries (rTYX rb)) \<and> rSY rb \<inter> set \<delta>Bc = {} \<and> distinct \<delta>Bc)"
-  proof -
-    obtain \<delta>xy where xy: "\<delta>xy = map (the \<circ> ring (rTYX rb')) (rb_incr_tail_n_delta \<delta>tl (rTXY rb'))"
-      by blast
-    obtain \<delta>yx where yx: "\<delta>yx = map (the \<circ> ring (rTYX rb)) (rb_incr_head_n_delta \<delta>hd (rTXY rb'))"
-      by blast 
-
-    from assms incr_tl rb_tl frame_weak_x_tl_delta 
-    have core1: "map (the \<circ> ring (rTXY rb')) (rb_valid_entries (rTXY rb')) = \<delta>xy @ map (the \<circ> ring (rTXY rb)) (rb_valid_entries (rTXY rb))" unfolding xy 
-      sorry
-    from assms incr_hd rb_hd frame_weak_x_hd_delta 
-    have core2: "map (the \<circ> ring (rTYX rb')) (rb_valid_entries (rTYX rb')) @ \<delta>yx = map (the \<circ> ring (rTYX rb)) (rb_valid_entries (rTYX rb))" unfolding yx
-      sorry
-
-  qed
-
-
-
+  have "map (the \<circ> ring (rTYX rb')) (rb_valid_entries (rTYX rb')) @ \<delta>yx = map (the \<circ> ring (rTYX rb)) (rb_valid_entries (rTYX rb))"
+    using I1 \<delta>yx_def frame frame_weak_x_hd_delta by blast
+  
+  have "rSY rb' \<union> set \<delta>xy = set \<delta>yx \<union> rSY rb "
+    
 
 qed
 *) 
